# Basics of Boolean Algebra
Many of the rules of Boolean algebra are fairly obvious. Even those that are not obvious can be verified easily by using a truth table. The figure below lists the most important of these laws. You will notice that all these laws, except the first, come in pairs: each law in the pair can be obtained from the other by interchanging $\wedge$ with $\vee$ and **T** with **F**. 

| Name                                     | Description                     |
| ---------------------------------------- | ------------------------------- |
| [[double negation law\|Double negation]] | ¬(¬p) ≡ p                       |
| [[excluded middle law\|Excluded middle]] | p ∨ ¬p ≡ T                      |
| [[contradiction law\|Contradiction]]     | p ∧ ¬p ≡ F                      |
| [[identity law\|Identity law]]           | T ∧ p ≡ p                       |
|                                          | F ∨ p ≡ p                       |
| [[idempotent law\|Idempotent laws]]      | p ∧ p ≡ p                       |
|                                          | p ∨ p ≡ p                       |
| [[commutative law\|Commutative laws]]    | p ∧ q ≡ q ∧ p                   |
|                                          | p ∨ q ≡ q ∨ p                   |
| [[associative law\|Associative laws]]    | (p ∧ q) ∧ r ≡ p ∧ (q ∧ r)       |
|                                          | (p ∨ q) ∨ r ≡ p ∨ (q ∨ r)       |
| [[distributive law\|Distributive laws]]  | p ∧ (q ∨ r) ≡ (p ∧ q) ∨ (p ∧ r) |
|                                          | p ∨ (q ∧ r) ≡ (p ∨ q) ∧ (p ∨ r) |
| [[De Morgan's law\|De Morgan's laws]]    | ¬(p ∧ q) ≡ (¬p) ∨ (¬q)          |
|                                          | ¬(p ∨ q) ≡ (¬p) ∧ (¬q)          |

Just as an example, let’s verify the first rule in the table, the Law of [[double negation law|Double negation]]. This law is just the basic grammar rule that two negatives make a positive.

| p   | ¬p  | ¬(¬p) | 
| --- | --- | ----- |
| 0   | 1   | 0     |
| 0   | 0   | 1     |

The fact that the first and last columns are identical shows the logical equivalence of p and $\neg$($\neg$p). The point here is not just that $\neg$($\neg$p) $\equiv$ p, but also that this logical equivalence is valid because it can be verified computationally based just on the relevant definitions. Its validity does not follow from the fact that “it’s obvious” or “it’s a well-known rule of grammar”.