# Simplifications
The final piece of algebra in Boolean algebra is the observation that we can chain logical equivalences together. That is, from P $\equiv$ Q and Q $\equiv$ R, it follows that P $\equiv$ R. This is really just a consequence of the [[Theorem 2.2 (Second Substitution Law)|Second Substitution Law]]. The equivalence Q $\equiv$ R allows us to substitute R for Q in the statement P $\equiv$ Q, giving P $\equiv$ R. (Remember that, by [[Definition 2.5]], logical equivalence is defined in terms of a proposition.) This means that we can show that two compound propositions are logically equivalent by finding a chain of logical equivalences that lead from one to the other. Here is an example of such a chain of logical equivalences:

p $\wedge$ (p $\rightarrow$ q) $\equiv$ p $\wedge$ ($\neg$p $\vee$ q) definition of p $\rightarrow$ q, [[Theorem 2.2 (Second Substitution Law)|Theorem 2.2]]
			$\equiv$ (p $\wedge$ $\neg$p) $\vee$ (p $\wedge$ q) [[distributive law|Distributive law]]
			$\equiv$ F $\vee$ (p $\wedge$ q) [[contradiction law|Law of Contradiction]], [[Theorem 2.2 (Second Substitution Law)|Theorem 2.2]]
			$\equiv$ (p $\wedge$ q) [[identity law|Identity Law]]

Each step in the chain has its own justification. In several cases, a substitution law is used without stating as much. In the first line, for example, the definition of p $\rightarrow$ q is that p $\rightarrow$ q $\equiv$ Â¬p $\vee$ q. [[Theorem 2.2 (Second Substitution Law)|The Second Substitution Law]] allows us to substitute $\neg$p $\vee$ q) for (p $\rightarrow$ q). In the last line, we implicitly applied the [[Theorem 2.1 (First Substitution Law)|First Substitution Law]] to the Identity Law, **F** $\vee$ p $\equiv$ p, to obtain **F** $\vee$ (p $\wedge$ q) $\equiv$ (p $\wedge$ q).

The chain of equivalences in the above example allows us to conclude that p $\wedge$ (p $\rightarrow$ q) is [[logically equivalent]] to p $\wedge$ q. This means that if you were to make a truth table for these two expressions, the truth values in the column for p $\wedge$ (p $\rightarrow$ q) would be identical to those in the column for p $\wedge$ q.

It takes practice to look at an expression and see which rules can be applied to it. For example, to see $\neg$(p $\vee$ q)) $\vee$ (p $\vee$ q) as an application of the law of the excluded middle for example, you need to mentally substitute (p $\vee$ q) for p in the law as it is stated in [[1. Basics of Boolean Algebra]]. Often, there are several rules that apply, and there are no definite guidelines about which one you should try. This is what makes algebra something of an art.