# More examples
The sum of an arbitrary number of terms is written using the symbol $\Sigma$. (This symbol is the Greek letter sigma, which is equivalent to the Latin letter S and stands for ‘sum’.) Thus, we have
$$\sum^5_{i=1}i^2 = 1^2 + 2^2 + 3^2 + 4^2 + 5^2$$
$$\sum^7_{k=3}a_k = a_3 + a_4 + a_5 + a_6 + a_7$$
$$\sum^N_{n=0}\frac{1}{n + 1} = \frac{1}{0 + 1} + \frac{1}{1 + 1} + \frac{1}{2 + 1} + ... + \frac{1}{N + 1}$$
This notation for a sum, using the $\Sigma$ operator, is called **summation notation**. A similar notation for products uses the symbol $\Pi$. (This is the Greek letter pi, which is equivalent to the Latin letter P and stands for ‘product’.) For example,
$$\prod^5_{k=2}(3k + 2) = (3 * 2 + 2)(3 * 3 + 2)(3 * 4 + 2)(3 * 5 + 2)$$
$$\prod^n_{i=1}\frac{1}{i} = \frac{1}{1} * \frac{1}{2} ... \frac{1}{n}$$
Induction can be used to prove many formulas that use these notations. Here are two examples:

### Theorem 3.7
$\sum^n_{i=1}i = \frac{n(n + 1)}{2}$ for any integer n greater than zero.

**Proof**. Let P(n) be the statement $\sum^n_{i=1}i = \frac{n(n + 1)}{2}$. We use induction to shwo that P(n) is true for all n > 0.
**Base case**: Consider the case n = 1. P(1) is the statement that $\sum^1_{i=1}i = \frac{1(1 + 1)}{2}$. Since each side of this equation is equal to one, this is true.
**Inductive case**: Let k $\geq$ 1 be arbitrary, and assume that P(k) is true. We want to show that P(k + 1) is true. P(k + 1) is the statement $\sum^{k+1}_{i=1}i = \frac{(k+1)((k+1) + 1)}{2}$. But, we can compute that

![[WhatsApp Image 2022-09-25 at 3.56.18 PM.jpeg]]

### Theorem 3.8
$\sum^n_{i=1}i2^i-1 = (n - 1) * 2^n + 1$ for any natural number n > 0.

**Proof**. Let P(n) be the statement $\sum^n_{i=1}i2^i-1 = (n - 1) * 2^n + 1$. We use induction
to show that P(n) is true for all n > 0.
**Base case**: Consider the case n = 1. P(1) is the statement that $\sum^1_{i=1}i2^{i-1} = (1 - 1) * 2^1 + 1$. Sinse each side of this equation is equal to one, this is true.
**Inductive case**: Let k $\geq$ 1 be arbitrary, and assume that P(k) is true. We want to show that P(k + 1) is true. P(k + 1) is the statement $\sum^{k+1}_{i=1}i2^{i-1} = ((k + 1) - 1) * 2^{k+1} + 1$. But, we can compute that
![[Pasted image 20220925151934.png]]
which is what we wanted to show. This completes the induction.