\section*{Solutions~3.2}%\ref{S-proof}}

\begin{solutions}
\setcounter{solutioncounter}{4}
\solution
The claim is: $(r \mid s) \wedge (s \mid t) \to r \mid t$.
\begin{proof}
	We need to show something is true for all integers $r, s, t$, so take arbitrary integers $k, m, n$ such that: $k \mid
	m$, $m \mid n$. \\
	Now we need to prove that $k \mid n$ holds.\\
	Since $k \mid m$, we know that $m = ak$ for some integer $a$. Similarly $n = bm$ for some integer $b$. \\
	Thus $n = bm = bak = ck$ with integer $c= ba$. \\
	Thus $k \mid n$.\\
	Since $k,m,n$ were arbitrary, this holds for all integers.
\end{proof}

\end{solutions}
